examples/SymEvalTest.v
@@ -27,7 +27,7 @@ Qed.
 Definition inc := MethodSig "inc"() : Void.
 Definition inc2 := MethodSig "inc2"() : Void.
 
-Notation SyntaxType k := (fullType (SyntaxKind k)).
+Notation SyntaxType k := (fullType type (SyntaxKind k)).
 
 Theorem really_atomic : forall rm o n dm cm, LtsStep (ConcatMod (MODULE {
                                                                      Register "r" : Bit 2 <- Default
